Watched_Literals: start correction of bounded IsaSAT without restart

Weidenbach_Book/Watched_Literals_Watch_List.thy
@@ -4737,4 +4737,91 @@ proof -
     done
 qed
 
+
+definition cdcl_twl_stgy_prog_early_wl :: \<open>'v twl_st_wl \<Rightarrow> (bool \<times> 'v twl_st_wl) nres\<close> where
+  \<open>cdcl_twl_stgy_prog_early_wl S\<^sub>0 =
+  do {
+    b \<leftarrow> SPEC(\<lambda>_. True);
+    (b, brk, T) \<leftarrow> WHILE\<^sub>T\<^bsup>\<lambda>(_, S). cdcl_twl_stgy_prog_wl_inv S\<^sub>0 S\<^esup>
+      (\<lambda>(b, brk, _). b \<and> \<not>brk)
+      (\<lambda>(_, brk, S). do {
+        T \<leftarrow> unit_propagation_outer_loop_wl S;
+        T \<leftarrow> cdcl_twl_o_prog_wl T;
+        b \<leftarrow> SPEC(\<lambda>_. True);
+        RETURN (b, T)
+      })
+      (b, False, S\<^sub>0);
+    RETURN (brk, T)
+  }\<close>
+
+theorem cdcl_twl_stgy_prog_early_wl_spec':
+  \<open>(cdcl_twl_stgy_prog_early_wl, cdcl_twl_stgy_prog_early_l) \<in> {(S::'v twl_st_wl, S').
+       (S, S') \<in> state_wl_l None \<and> correct_watching S} \<rightarrow>\<^sub>f
+    \<langle>bool_rel \<times>\<^sub>r {(S::'v twl_st_wl, S'). (S, S') \<in> state_wl_l None \<and> correct_watching S}\<rangle>nres_rel\<close>
+   (is \<open>?o \<in> ?A \<rightarrow>\<^sub>f \<langle>?B\<rangle> nres_rel\<close>)
+proof -
+  have H: \<open>((b', False, S'), b, False, S) \<in> {((b', brk', T'), (b, brk, T)).
+      (T', T) \<in> state_wl_l None \<and> brk' = brk \<and> b' = b \<and>
+       correct_watching T'}\<close>
+    if \<open>(S', S) \<in> state_wl_l None\<close> and
+       \<open>correct_watching S'\<close> and
+       \<open>(b', b) \<in> bool_rel\<close>
+    for S' :: \<open>'v twl_st_wl\<close> and S :: \<open>'v twl_st_l\<close> and b' b :: bool
+    using that by auto
+  show ?thesis
+    unfolding cdcl_twl_stgy_prog_early_wl_def cdcl_twl_stgy_prog_early_l_def fref_param1[symmetric]
+    apply (refine_rcg H unit_propagation_outer_loop_wl_spec[THEN fref_to_Down]
+      cdcl_twl_o_prog_wl_spec[THEN fref_to_Down]
+      cdcl_twl_stgy_prog_wl_spec'[unfolded fref_param1, THEN fref_to_Down])
+    subgoal for S' S by (cases S') auto
+    subgoal by auto
+    subgoal unfolding cdcl_twl_stgy_prog_wl_inv_def by blast
+    subgoal by auto
+    subgoal by auto
+    subgoal for S' S brk'T' brkT brk' T' by auto
+    subgoal by fast
+    subgoal by auto
+    subgoal by auto
+    done
+qed
+
+
+theorem cdcl_twl_stgy_prog_early_wl_spec:
+  \<open>(cdcl_twl_stgy_prog_early_wl, cdcl_twl_stgy_prog_early_l) \<in> {(S::'v twl_st_wl, S').
+       (S, S') \<in> state_wl_l None \<and>
+       correct_watching S} \<rightarrow>\<^sub>f
+    \<langle>bool_rel \<times>\<^sub>r state_wl_l None\<rangle>nres_rel\<close>
+   (is \<open>?o \<in> ?A \<rightarrow>\<^sub>f \<langle>?B\<rangle> nres_rel\<close>)
+  using cdcl_twl_stgy_prog_early_wl_spec'
+  apply -
+  apply (rule mem_set_trans)
+  prefer 2 apply assumption
+  apply (match_fun_rel, solves simp)
+  apply (match_fun_rel; solves auto)
+  done
+
+lemma cdcl_twl_stgy_prog_early_wl_spec_final:
+  assumes
+    \<open>cdcl_twl_stgy_prog_wl_pre S S'\<close>
+  shows
+    \<open>cdcl_twl_stgy_prog_early_wl S \<le> \<Down> (bool_rel \<times>\<^sub>r (state_wl_l None O twl_st_l None)) (partial_conclusive_TWL_run S')\<close>
+proof -
+  obtain T where T: \<open>(S, T) \<in> state_wl_l None\<close> \<open>cdcl_twl_stgy_prog_l_pre T S'\<close> \<open>correct_watching S\<close>
+    using assms unfolding cdcl_twl_stgy_prog_wl_pre_def by blast
+  have H: \<open>{((a, b), a', b'). (a, a') \<in> bool_rel \<and> (b, b') \<in> state_wl_l None} O
+       (bool_rel \<times>\<^sub>f twl_st_l None) = bool_rel \<times>\<^sub>r  state_wl_l None O twl_st_l None\<close>
+    by fastforce
+  show ?thesis
+    apply (rule order_trans[OF cdcl_twl_stgy_prog_early_wl_spec[unfolded fref_param1[symmetric], "to_\<Down>", of S T]])
+    subgoal using T by auto
+    subgoal
+      apply (rule order_trans)
+      apply (rule ref_two_step')
+       apply (rule cdcl_twl_stgy_prog_early_l_spec_final[of _ S'])
+      subgoal using T by fast
+      subgoal unfolding H conc_fun_chain by auto
+      done
+    done
+qed
+
 end
