Weidenbach_Book/Watched_Literals_Watch_List_Domain.thy
@@ -1952,4 +1952,45 @@ text \<open>The definition is here to be shared later.\<close>
 definition get_propagation_reason :: \<open>('v, 'mark) ann_lits \<Rightarrow> 'v literal \<Rightarrow> 'mark option nres\<close> where
   \<open>get_propagation_reason M L = SPEC(\<lambda>C. C \<noteq> None \<longrightarrow> Propagated L (the C) \<in> set M)\<close>
 
+definition cdcl_twl_stgy_prog_bounded_wl_D_heur :: \<open>twl_st_wl_heur \<Rightarrow> (bool \<times> twl_st_wl_heur) nres\<close>
+where
+  \<open>cdcl_twl_stgy_prog_bounded_wl_D_heur S\<^sub>0 =
+  do {
+    b \<leftarrow> RETURN (isasat_fast S\<^sub>0);
+    (b, brk, T) \<leftarrow> WHILE\<^sub>T\<^bsup>\<lambda>(b, brk, T). True\<^esup>
+        (\<lambda>(b, brk, _). b \<and> \<not>brk)
+        (\<lambda>(b, brk, S).
+        do {
+          ASSERT(isasat_fast S);
+          T \<leftarrow> unit_propagation_outer_loop_wl_D_heur S;
+          ASSERT(isasat_fast T);
+          (brk, T) \<leftarrow> cdcl_twl_o_prog_wl_D_heur T;
+          b \<leftarrow> RETURN (isasat_fast T);
+          RETURN(b, brk, T)
+        })
+        (b, False, S\<^sub>0);
+    RETURN (b, T)
+  }\<close>
+
+lemma cdcl_twl_stgy_prog_break_wl_D_spec_final:
+  assumes
+    \<open>cdcl_twl_stgy_prog_wl_D_pre S S'\<close>
+  shows
+    \<open>cdcl_twl_stgy_prog_break_wl_D S \<le> \<Down> (state_wl_l None O twl_st_l None) (conclusive_TWL_run S')\<close>
+proof -
+  have T: \<open>cdcl_twl_stgy_prog_wl_pre S S' \<and> literals_are_\<L>\<^sub>i\<^sub>n (all_atms_st S) S\<close>
+    using assms unfolding cdcl_twl_stgy_prog_wl_D_pre_def by blast
+  show ?thesis
+    apply (rule order_trans[OF cdcl_twl_stgy_prog_break_wl_D_spec[of \<open>all_atms_st S\<close>]])
+    subgoal using T by auto
+    subgoal
+      apply (rule order_trans)
+      apply (rule ref_two_step')
+       apply (rule cdcl_twl_stgy_prog_break_wl_spec_final[of _ S'])
+      subgoal using T by fast
+      subgoal unfolding conc_fun_chain by (rule conc_fun_R_mono) blast
+      done
+    done
+qed
+
 end
